tutorial/utp_csp_mini_mondex.thy
@@ -108,7 +108,7 @@ lemma Pay_contract [rdes_def]:
             \<triangleleft> \<guillemotleft>i\<guillemotright> \<notin>\<^sub>u dom\<^sub>u(&accts) \<or> \<guillemotleft>n\<guillemotright> \<le>\<^sub>u 0 \<or> &accts(\<guillemotleft>i\<guillemotright>)\<^sub>a <\<^sub>u \<guillemotleft>n\<guillemotright> \<triangleright>\<^sub>R
           \<Phi>(true,[&accts \<mapsto>\<^sub>s &accts(\<guillemotleft>i\<guillemotright> \<mapsto> &accts(\<guillemotleft>i\<guillemotright>)\<^sub>a - \<guillemotleft>n\<guillemotright>, \<guillemotleft>j\<guillemotright> \<mapsto> &accts(\<guillemotleft>j\<guillemotright>)\<^sub>a + \<guillemotleft>n\<guillemotright>)\<^sub>u]
                 ,\<langle>(pay\<cdot>(\<guillemotleft>i\<guillemotright>, \<guillemotleft>j\<guillemotright>, \<guillemotleft>n\<guillemotright>)\<^sub>u)\<^sub>u, (accept\<cdot>\<guillemotleft>i\<guillemotright>)\<^sub>u\<rangle>)))"
-  using assms by (simp add: Pay_def closure, rdes_simp)  
+  using assms by (simp add: Pay_def closure, rdes_simp, simp add: pr_var_def)  
 
 lemma Pay_contract':
   assumes "i \<noteq> j"
@@ -127,9 +127,9 @@ lemma Pay_contract':
             \<triangleleft> \<guillemotleft>i\<guillemotright> \<notin>\<^sub>u dom\<^sub>u(&accts) \<or> \<guillemotleft>n\<guillemotright> \<le>\<^sub>u 0 \<or> &accts(\<guillemotleft>i\<guillemotright>)\<^sub>a <\<^sub>u \<guillemotleft>n\<guillemotright> \<triangleright>\<^sub>R
           (&tt =\<^sub>u \<langle>(pay\<cdot>(\<guillemotleft>i\<guillemotright>, \<guillemotleft>j\<guillemotright>, \<guillemotleft>n\<guillemotright>)\<^sub>u)\<^sub>u, (accept\<cdot>\<guillemotleft>i\<guillemotright>)\<^sub>u\<rangle> \<and>
              [\<langle>[&accts \<mapsto>\<^sub>s &accts(\<guillemotleft>i\<guillemotright> \<mapsto> &accts(\<guillemotleft>i\<guillemotright>)\<^sub>a - \<guillemotleft>n\<guillemotright>
-                                , \<guillemotleft>j\<guillemotright> \<mapsto> &accts(\<guillemotleft>j\<guillemotright>)\<^sub>a + \<guillemotleft>n\<guillemotright>)\<^sub>u]\<rangle>\<^sub>a]\<^sub>S
+                                , \<guillemotleft>j\<guillemotright> \<mapsto> &accts(\<guillemotleft>j\<guillemotright>)\<^sub>a + \<guillemotleft>n\<guillemotright>)\<^sub>u]\<rangle>\<^sub>a]\<^sub>S'
           )))"
-  using assms by (simp add: Pay_def closure, rdes_simp, rel_auto)  
+  using assms by (simp add: Pay_def closure, rdes_simp, rel_auto) 
     
 lemma Pay_wf [closure]:
   "Pay i j n is NCSP"
@@ -163,7 +163,7 @@ text {* We perform verification by writing contracts that specify desired behavi
   that initially the number of cards is $cardNum$. The pericondition is $true$ as we don't
   care about intermediate behaviour here. The postcondition has that the summation of the 
   sequence of card values remains the same, though of course individual records will change. *}
-     
+  
 theorem money_constant:
   assumes "finite cards" "i \<in> cards" "j \<in> cards" "i \<noteq> j" 
   shows "[dom\<^sub>u(&accts) =\<^sub>u \<guillemotleft>cards\<guillemotright> \<turnstile> true | sum\<^sub>u($accts) =\<^sub>u sum\<^sub>u($accts\<acute>)]\<^sub>C \<sqsubseteq> Pay i j n"
@@ -198,11 +198,11 @@ proof (simp add: assms Pay_contract, rule CRD_refine_rdes)
     be retrieved by sledgehammer. However, we actually had to prove that property first and add it to our library. *}
       
   from assms
-  show "[sum\<^sub>u($accts) =\<^sub>u sum\<^sub>u($accts\<acute>)]\<^sub>S\<lbrakk>x\<rightarrow>&tt\<rbrakk> \<sqsubseteq>
+  show "[sum\<^sub>u($accts) =\<^sub>u sum\<^sub>u($accts\<acute>)]\<^sub>S'\<lbrakk>x\<rightarrow>&tt\<rbrakk> \<sqsubseteq>
     ([dom\<^sub>u(&accts) =\<^sub>u \<guillemotleft>cards\<guillemotright>]\<^sub>S\<^sub>< \<and>
      \<Phi>(true,id,\<langle>(pay\<cdot>(\<guillemotleft>i\<guillemotright>, \<guillemotleft>j\<guillemotright>, \<guillemotleft>n\<guillemotright>)\<^sub>u)\<^sub>u, (reject\<cdot>\<guillemotleft>i\<guillemotright>)\<^sub>u\<rangle>) \<triangleleft> \<guillemotleft>i\<guillemotright> \<notin>\<^sub>u dom\<^sub>u(&accts) \<or> \<guillemotleft>n\<guillemotright> \<le>\<^sub>u 0 \<or> &accts(\<guillemotleft>i\<guillemotright>)\<^sub>a <\<^sub>u \<guillemotleft>n\<guillemotright> \<triangleright>\<^sub>R
         \<Phi>(true,[&accts \<mapsto>\<^sub>s &accts(\<guillemotleft>i\<guillemotright> \<mapsto> &accts(\<guillemotleft>i\<guillemotright>)\<^sub>a - \<guillemotleft>n\<guillemotright>, \<guillemotleft>j\<guillemotright> \<mapsto> &accts(\<guillemotleft>j\<guillemotright>)\<^sub>a + \<guillemotleft>n\<guillemotright>)\<^sub>u],\<langle>(pay\<cdot>(\<guillemotleft>i\<guillemotright>, \<guillemotleft>j\<guillemotright>, \<guillemotleft>n\<guillemotright>)\<^sub>u)\<^sub>u, (accept\<cdot>\<guillemotleft>i\<guillemotright>)\<^sub>u\<rangle>))"
-    by (rel_simp, simp add: pfun_sums_upd_2)
+    by (rel_auto, simp_all add: pfun_sums_upd_2)
 qed
       
 text {* The next property is that no card value can go below 0, assuming it was non-zero to start
